semantics/typeSystemScript.sml
@@ -785,9 +785,9 @@ val _ = Define `
  (tscheme_inst2 _ ts1 ts2 = (tscheme_inst ts1 ts2))`;
 
 
-(*val weak_tenv : list modN -> type_env -> type_env -> bool*)
+(*val weak_tenv : type_env -> type_env -> bool*)
 val _ = Define `
- (weak_tenv mn tenv_impl tenv_spec =  
+ (weak_tenv tenv_impl tenv_spec =  
 (eSubEnv tscheme_inst2 tenv_spec.v tenv_impl.v /\
   eSubEnv (\i x y .  (case (i ,x ,y ) of ( _ , x , y ) => x = y )) tenv_spec.c tenv_impl.c /\
   eSubEnv weak_tenvT tenv_spec.t tenv_impl.t))`;
@@ -799,7 +799,7 @@ T
 check_signature mn tenvT decls tenv NONE decls tenv)
 
 /\ (! mn specs tenv_impl tenv_spec decls_impl decls_spec tenvT.
-(weak_tenv mn tenv_impl tenv_spec /\
+(weak_tenv tenv_impl tenv_spec /\
 weak_decls decls_impl decls_spec /\
 type_specs mn tenvT specs decls_spec tenv_spec)
 ==>
